Trying to remove the link from frames -- the stack abstraction should be used instead.

backend/Asmgenproof0.v
@@ -317,6 +317,8 @@ Section WITHEXTERNALCALLS.
 Context `{external_calls_prf: ExternalCalls}.
 Context {injperm: InjectPerm}.
 
+Variable init_sp: val.
+
 Lemma extcall_arg_match:
   forall ms sp rs m m' l v,
   agree ms sp rs ->
@@ -765,12 +767,12 @@ Inductive exec_straight: code -> regset -> mem ->
                          code -> regset -> mem -> Prop :=
   | exec_straight_one:
       forall i1 c rs1 m1 rs2 m2,
-      exec_instr ge fn i1 rs1 m1 = Next rs2 m2 ->
+      exec_instr init_sp ge fn i1 rs1 m1 = Next rs2 m2 ->
       rs2#PC = Val.offset_ptr rs1#PC Ptrofs.one ->
       exec_straight (i1 :: c) rs1 m1 c rs2 m2
   | exec_straight_step:
       forall i c rs1 m1 rs2 m2 c' rs3 m3,
-      exec_instr ge fn i rs1 m1 = Next rs2 m2 ->
+      exec_instr init_sp ge fn i rs1 m1 = Next rs2 m2 ->
       rs2#PC = Val.offset_ptr rs1#PC Ptrofs.one ->
       exec_straight c rs2 m2 c' rs3 m3 ->
       exec_straight (i :: c) rs1 m1 c' rs3 m3.
@@ -788,8 +790,8 @@ Qed.
 
 Lemma exec_straight_two:
   forall i1 i2 c rs1 m1 rs2 m2 rs3 m3,
-  exec_instr ge fn i1 rs1 m1 = Next rs2 m2 ->
-  exec_instr ge fn i2 rs2 m2 = Next rs3 m3 ->
+  exec_instr init_sp ge fn i1 rs1 m1 = Next rs2 m2 ->
+  exec_instr init_sp ge fn i2 rs2 m2 = Next rs3 m3 ->
   rs2#PC = Val.offset_ptr rs1#PC Ptrofs.one ->
   rs3#PC = Val.offset_ptr rs2#PC Ptrofs.one ->
   exec_straight (i1 :: i2 :: c) rs1 m1 c rs3 m3.
@@ -800,9 +802,9 @@ Qed.
 
 Lemma exec_straight_three:
   forall i1 i2 i3 c rs1 m1 rs2 m2 rs3 m3 rs4 m4,
-  exec_instr ge fn i1 rs1 m1 = Next rs2 m2 ->
-  exec_instr ge fn i2 rs2 m2 = Next rs3 m3 ->
-  exec_instr ge fn i3 rs3 m3 = Next rs4 m4 ->
+  exec_instr init_sp ge fn i1 rs1 m1 = Next rs2 m2 ->
+  exec_instr init_sp ge fn i2 rs2 m2 = Next rs3 m3 ->
+  exec_instr init_sp ge fn i3 rs3 m3 = Next rs4 m4 ->
   rs2#PC = Val.offset_ptr rs1#PC Ptrofs.one ->
   rs3#PC = Val.offset_ptr rs2#PC Ptrofs.one ->
   rs4#PC = Val.offset_ptr rs3#PC Ptrofs.one ->
@@ -823,7 +825,7 @@ Lemma exec_straight_steps_1:
   rs#PC = Vptr b ofs ->
   Genv.find_funct_ptr ge b = Some (Internal fn) ->
   code_tail (Ptrofs.unsigned ofs) (fn_code fn) c ->
-  plus step ge (State rs m) E0 (State rs' m').
+  plus (step init_sp) ge (State rs m) E0 (State rs' m').
 Proof.
   induction 1; intros.
   apply plus_one.
@@ -866,7 +868,7 @@ End STRAIGHTLINE.
 
 Section MATCH_STACK.
 
-Variables init_sp init_ra: val.
+Variables init_ra: val.
 Hypothesis init_sp_not_vundef: init_sp <> Vundef.
 Hypothesis init_ra_not_vundef: init_ra <> Vundef.
 Hypothesis init_sp_type: Val.has_type init_sp Tptr.
