x86/Stacklayout.v
@@ -33,14 +33,14 @@ Definition fe_ofs_arg := 0.
 
 Definition make_env (b: bounds) : frame_env :=
   let w := if Archi.ptr64 then 8 else 4 in
-  let olink := align (4 * b.(bound_outgoing)) w in  (* back link *)
-  let ocs := olink + w in                           (* callee-saves *)
+  let ocs := align (4 * b.(bound_outgoing)) w in  (* back link *)
+  (* let ocs := olink + w in                           (* callee-saves *) *)
   let ol :=  align (size_callee_save_area b ocs) 8 in (* locals *)
   let ostkdata := align (ol + 4 * b.(bound_local)) 8 in (* stack data *)
   let oretaddr := align (ostkdata + b.(bound_stack_data)) w in (* return address *)
   let sz := oretaddr + w in (* total size *)
   {| fe_size := sz;
-     fe_ofs_link := olink;
+     (* fe_ofs_link := olink; *)
      fe_ofs_retaddr := oretaddr;
      fe_ofs_local := ol;
      fe_ofs_callee_save := ocs;
@@ -55,7 +55,7 @@ Section WITHMEM.
       m |= range sp 0 (fe_stack_data fe) ** range sp (fe_stack_data fe + bound_stack_data b) (fe_size fe) ** P ->
       m |= range sp (fe_ofs_local fe) (fe_ofs_local fe + 4 * bound_local b)
         ** range sp fe_ofs_arg (fe_ofs_arg + 4 * bound_outgoing b)
-        ** range sp (fe_ofs_link fe) (fe_ofs_link fe + size_chunk Mptr)
+        (* ** range sp (fe_ofs_link fe) (fe_ofs_link fe + size_chunk Mptr) *)
         ** range sp (fe_ofs_retaddr fe) (fe_ofs_retaddr fe + size_chunk Mptr)
         ** range sp (fe_ofs_callee_save fe) (size_callee_save_area b (fe_ofs_callee_save fe))
         ** P.
@@ -63,8 +63,8 @@ Section WITHMEM.
     Local Opaque Z.add Z.mul sepconj range.
     intros; simpl.
     set (w := if Archi.ptr64 then 8 else 4).
-    set (olink := align (4 * b.(bound_outgoing)) w).
-    set (ocs := olink + w).
+    set (ocs := align (4 * b.(bound_outgoing)) w).
+    (* set (ocs := olink + w). *)
     set (ol :=  align (size_callee_save_area b ocs) 8).
     set (ostkdata := align (ol + 4 * b.(bound_local)) 8).
     set (oretaddr := align (ostkdata + b.(bound_stack_data)) w).
@@ -72,26 +72,25 @@ Section WITHMEM.
     assert (0 < w) by (unfold w; destruct Archi.ptr64; omega).
     generalize b.(bound_local_pos) b.(bound_outgoing_pos) b.(bound_stack_data_pos); intros.
     assert (0 <= 4 * b.(bound_outgoing)) by omega.
-    assert (4 * b.(bound_outgoing) <= olink) by (apply align_le; omega).
-    assert (olink + w <= ocs) by (unfold ocs; omega).
+    assert (4 * b.(bound_outgoing) <= ocs) by (apply align_le; omega).
+    (* assert (olink + w <= ocs) by (unfold ocs; omega). *)
     assert (ocs <= size_callee_save_area b ocs) by (apply size_callee_save_area_incr). 
     assert (size_callee_save_area b ocs <= ol) by (apply align_le; omega).
     assert (ol + 4 * b.(bound_local) <= ostkdata) by (apply align_le; omega).
     assert (ostkdata + bound_stack_data b <= oretaddr) by (apply align_le; omega).
     (* Reorder as:
      outgoing
-     back link
      callee-save
      local
      retaddr *)
     rewrite sep_swap12.
     rewrite sep_swap23.
-    rewrite sep_swap45.
+    rewrite sep_swap34.
+    rewrite sep_swap23.
     rewrite sep_swap34.
     (* Apply range_split and range_split2 repeatedly *)
     unfold fe_ofs_arg.
-    apply range_split_2. fold olink. omega. omega. 
-    apply range_split. omega.
+    apply range_split_2. fold ocs. omega. omega. 
     apply range_split_2. fold ol. omega. omega.
     apply range_drop_right with ostkdata. omega.
     rewrite sep_swap.
@@ -105,18 +104,18 @@ Lemma frame_env_separated':
   forall b ,
     let w := if Archi.ptr64 then 8 else 4 in
     let fe := make_env b in
-     let olink := align (4 * bound_outgoing b) w in
-     let ocs := olink + w in
+     let ocs := align (4 * bound_outgoing b) w in
+     (* let ocs := olink + w in *)
      let ol := align (size_callee_save_area b ocs) 8 in
      let ostkdata := align (ol + 4 * bound_local b) 8 in
      let oretaddr := align (ostkdata + bound_stack_data b) w in
-     0 <= olink
-  /\ olink + w <= ocs
+     0 <= ocs
+  (* /\ olink + w <= ocs *)
   /\ ocs <= size_callee_save_area b ocs
   /\ size_callee_save_area b ocs <= ol
   /\ ol + 4 * bound_local b <= ostkdata
   /\ ostkdata + bound_stack_data b <= oretaddr
-  /\ olink <= fe_stack_data fe.
+  /\ ocs <= fe_stack_data fe.
 Proof.
 Local Opaque Z.add Z.mul sepconj range fe_stack_data.
 intros; simpl.
@@ -125,8 +124,8 @@ replace (size_chunk Mptr) with w by (rewrite size_chunk_Mptr; auto).
 assert (0 < w) by (unfold w; destruct Archi.ptr64; omega).
 generalize b.(bound_local_pos) b.(bound_outgoing_pos) b.(bound_stack_data_pos); intros.
 assert (0 <= 4 * b.(bound_outgoing)) by omega.
-assert (4 * b.(bound_outgoing) <= olink) by (apply align_le; omega).
-assert (olink + w <= ocs) by (unfold ocs; omega).
+assert (4 * b.(bound_outgoing) <= ocs) by (apply align_le; omega).
+(* assert (olink + w <= ocs) by (unfold ocs; omega). *)
 assert (ocs <= size_callee_save_area b ocs) by (apply size_callee_save_area_incr). 
 assert (size_callee_save_area b ocs <= ol) by (apply align_le; omega).
 assert (ol + 4 * b.(bound_local) <= ostkdata) by (apply align_le; omega).
@@ -134,7 +133,7 @@ assert (ostkdata + bound_stack_data b <= oretaddr) by (apply align_le; omega).
 repeat split; auto.
 omega.
 Local Transparent fe_stack_data.
-simpl. fold w. fold olink. fold ocs. fold ol. fold ostkdata. omega.
+simpl. fold w. fold ocs. fold ol. fold ostkdata. omega.
 Qed.
 
 Lemma frame_env_range:
@@ -144,16 +143,15 @@ Lemma frame_env_range:
 Proof.
   intros; simpl.
   set (w := if Archi.ptr64 then 8 else 4).
-  set (olink := align (4 * b.(bound_outgoing)) w).
-  set (ocs := olink + w).
+  set (ocs := align (4 * b.(bound_outgoing)) w).
+  (* set (ocs := olink + w). *)
   set (ol :=  align (size_callee_save_area b ocs) 8).
   set (ostkdata := align (ol + 4 * b.(bound_local)) 8).
   set (oretaddr := align (ostkdata + b.(bound_stack_data)) w).
   assert (0 < w) by (unfold w; destruct Archi.ptr64; omega).
   generalize b.(bound_local_pos) b.(bound_outgoing_pos) b.(bound_stack_data_pos); intros.
   assert (0 <= 4 * b.(bound_outgoing)) by omega.
-  assert (4 * b.(bound_outgoing) <= olink) by (apply align_le; omega).
-  assert (olink + w <= ocs) by (unfold ocs; omega).
+  assert (4 * b.(bound_outgoing) <= ocs) by (apply align_le; omega).
   assert (ocs <= size_callee_save_area b ocs) by (apply size_callee_save_area_incr). 
   assert (size_callee_save_area b ocs <= ol) by (apply align_le; omega).
   assert (ol + 4 * b.(bound_local) <= ostkdata) by (apply align_le; omega).
@@ -167,20 +165,18 @@ Lemma frame_env_aligned:
      (8 | fe_ofs_arg)
   /\ (8 | fe_ofs_local fe)
   /\ (8 | fe_stack_data fe)
-  /\ (align_chunk Mptr | fe_ofs_link fe)
+  (* /\ (align_chunk Mptr | fe_ofs_link fe) *)
   /\ (align_chunk Mptr | fe_ofs_retaddr fe).
 Proof.
   intros; simpl.
   set (w := if Archi.ptr64 then 8 else 4).
-  set (olink := align (4 * b.(bound_outgoing)) w).
-  set (ocs := olink + w).
+  set (ocs := align (4 * b.(bound_outgoing)) w).
   set (ol :=  align (size_callee_save_area b ocs) 8).
   set (ostkdata := align (ol + 4 * b.(bound_local)) 8).
   set (oretaddr := align (ostkdata + b.(bound_stack_data)) w).
   assert (0 < w) by (unfold w; destruct Archi.ptr64; omega).
   replace (align_chunk Mptr) with w by (rewrite align_chunk_Mptr; auto).
   split. apply Zdivide_0.
-  split. apply align_divides; omega.
   split. apply align_divides; omega.
   split. apply align_divides; omega.
   apply align_divides; omega.
@@ -211,45 +207,42 @@ Program Definition frame_of_frame_env (b: bounds) : frame_info :=
   let fe := make_env b in
   {|
     frame_size := fe_size fe;
-    frame_link := {| seg_ofs := (fe_ofs_link fe); seg_size := size_chunk Mptr |} :: nil;
+    frame_link := nil;
     frame_perm := fun o =>
                     if zle (fe_ofs_retaddr fe) o && zlt o (fe_ofs_retaddr fe + size_chunk Mptr)
                     then Readonly
                     else
-                      if zle (fe_ofs_link fe) o && zlt o (fe_ofs_link fe + size_chunk Mptr)
-                      then Readonly
+                      if zle (fe_ofs_local fe) o && zlt o (fe_ofs_local fe + 4 * bound_local b)
+                      then Private
                       else
-                        if zle (fe_ofs_local fe) o && zlt o (fe_ofs_local fe + 4 * bound_local b)
+                        if zle (fe_ofs_arg) o && zlt o (fe_ofs_arg + 4 * bound_outgoing b)
                         then Private
                         else
-                          if zle (fe_ofs_arg) o && zlt o (fe_ofs_arg + 4 * bound_outgoing b)
+                          if zle (fe_ofs_callee_save fe) o && zlt o (size_callee_save_area b (fe_ofs_callee_save fe))
                           then Private
-                          else
-                            if zle (fe_ofs_callee_save fe) o && zlt o (size_callee_save_area b (fe_ofs_callee_save fe))
-                            then Private
-                            else Public
+                          else Public
   |}.
-Next Obligation.
-  rewrite Forall_forall. intros ? [?|[]]; subst. intros i H. simpl in *.
-  split. etransitivity. 2: apply H.
-  etransitivity. 2: apply align_le. generalize (bound_outgoing_pos b); omega.
-  destr; omega.
-  eapply Zlt_le_trans. apply H.
-  etransitivity. 2: apply le_add_pos. 2: destr; omega.
-  etransitivity. 2: apply align_le. 2: destr; omega.
-  etransitivity. 2: apply le_add_pos. 2: generalize (bound_stack_data_pos b); omega.
-  etransitivity. 2: apply align_le. 2: omega. 
-  etransitivity. 2: apply le_add_pos. 2: generalize (bound_local_pos b); omega.
-  etransitivity. 2: apply align_le. 2: omega.
-  change (size_chunk Mptr) with (if Archi.ptr64 then 8 else 4).
-  apply size_callee_save_area_incr.
-Qed.
-Next Obligation.
-  rewrite Forall_forall. intros ? [?|[]]; subst. intros i H.
-  red in H. simpl in *.
-  rewrite ! and_sumbool.
-  repeat destr.
-Qed.
+(* Next Obligation. *)
+(*   rewrite Forall_forall. intros ? [?|[]]; subst. intros i H. simpl in *. *)
+(*   split. etransitivity. 2: apply H. *)
+(*   etransitivity. 2: apply align_le. generalize (bound_outgoing_pos b); omega. *)
+(*   destr; omega. *)
+(*   eapply Zlt_le_trans. apply H. *)
+(*   etransitivity. 2: apply le_add_pos. 2: destr; omega. *)
+(*   etransitivity. 2: apply align_le. 2: destr; omega. *)
+(*   etransitivity. 2: apply le_add_pos. 2: generalize (bound_stack_data_pos b); omega. *)
+(*   etransitivity. 2: apply align_le. 2: omega.  *)
+(*   etransitivity. 2: apply le_add_pos. 2: generalize (bound_local_pos b); omega. *)
+(*   etransitivity. 2: apply align_le. 2: omega. *)
+(*   change (size_chunk Mptr) with (if Archi.ptr64 then 8 else 4). *)
+(*   apply size_callee_save_area_incr. *)
+(* Qed. *)
+(* Next Obligation. *)
+(*   rewrite Forall_forall. intros ? [?|[]]; subst. intros i H. *)
+(*   red in H. simpl in *. *)
+(*   rewrite ! and_sumbool. *)
+(*   repeat destr. *)
+(* Qed. *)
 
 Lemma stkdata_retaddr_sep:
   forall b,
@@ -276,35 +269,14 @@ Proof.
   generalize (frame_env_separated' b).
   simpl. intuition.
   cut (o<o). omega.
-  eapply Z.lt_le_trans. apply H9.
-  etransitivity. 2: apply H5.
+  eapply Z.lt_le_trans. apply H8.
+  etransitivity. 2: apply H4.
   etransitivity. 2: apply align_le; try (destr; omega).
   etransitivity. 2: apply le_add_pos; try (generalize (bound_stack_data_pos b); omega).
   etransitivity. 2: apply align_le; try (omega).
   etransitivity. 2: apply le_add_pos; try (generalize (bound_local_pos b); omega).
   etransitivity. 2: apply align_le; try (omega).
   etransitivity. 2: apply size_callee_save_area_incr.
-  etransitivity. 2: apply le_add_pos; try (destr; omega).
-  change fe_ofs_arg with 0.
-  rewrite Z.add_0_l.
-  apply align_le. destr; omega.
-Qed.
-
-
-Lemma arg_link_sep:
-  forall b,
-    let fe := make_env b in
-    forall o,
-      fe_ofs_arg <= o < fe_ofs_arg + 4 * bound_outgoing b ->
-      fe_ofs_link fe <= o < fe_ofs_link fe + size_chunk Mptr ->
-      False.
-Proof.
-  clear. intros b fe.
-  generalize (frame_env_separated' b).
-  simpl. intuition.
-  cut (o<o). omega.
-  eapply Z.lt_le_trans. apply H9.
-  etransitivity. 2: apply H5.
   change fe_ofs_arg with 0.
   rewrite Z.add_0_l.
   apply align_le. destr; omega.
@@ -322,16 +294,14 @@ Proof.
   generalize (frame_env_separated' b).
   simpl. intuition.
   cut (o<o). omega.
-  eapply Z.lt_le_trans. apply H9.
-  etransitivity. 2: apply H5.
+  eapply Z.lt_le_trans. apply H8.
+  etransitivity. 2: apply H4.
   etransitivity. 2: apply align_le; try (omega).
   etransitivity. 2: apply size_callee_save_area_incr.
-  etransitivity. 2: apply le_add_pos; try (destr; omega).
   change fe_ofs_arg with 0.
   rewrite Z.add_0_l.
   apply align_le. destr; omega.
 Qed.
-
 
 Lemma arg_callee_save_sep:
   forall b,
@@ -345,14 +315,12 @@ Proof.
   generalize (frame_env_separated' b).
   simpl. intuition.
   cut (o<o). omega.
-  eapply Z.lt_le_trans. apply H9.
-  etransitivity. 2: apply H5.
-  etransitivity. 2: apply le_add_pos; try (destr; omega).
+  eapply Z.lt_le_trans. apply H8.
+  etransitivity. 2: apply H4.
   change fe_ofs_arg with 0.
   rewrite Z.add_0_l.
   apply align_le. destr; omega.
 Qed.
-
 
 Lemma local_retaddr_sep:
   forall b,
@@ -366,53 +334,12 @@ Proof.
   generalize (frame_env_separated' b).
   simpl. intuition.
   cut (o < o). omega.
-  eapply Z.lt_le_trans. apply H9.
-  etransitivity. 2: apply H5.
+  eapply Z.lt_le_trans. apply H8.
+  etransitivity. 2: apply H4.
   etransitivity. 2: apply align_le; try (destr; omega).
   etransitivity. 2: apply le_add_pos; try (generalize (bound_stack_data_pos b); omega).
   apply align_le; try (omega).
 Qed.
-
-Lemma local_link_sep:
-  forall b,
-    let fe := make_env b in
-    forall o,
-      fe_ofs_local fe <= o < fe_ofs_local fe + 4 * bound_local b ->
-      fe_ofs_link fe <= o < fe_ofs_link fe + size_chunk Mptr ->
-      False.
-Proof.
-  clear. intros b fe.
-  generalize (frame_env_separated' b).
-  simpl. intuition.
-  cut (o < o). omega.
-  eapply Z.lt_le_trans. apply H10.
-  etransitivity. 2: apply H8.
-  etransitivity. 2: apply align_le; try (omega).
-  etransitivity. 2:   apply size_callee_save_area_incr.
-  unfold Mptr. destr.
-Qed.
-
-Lemma stkdata_link_sep:
-  forall b,
-    let fe := make_env b in
-    forall o,
-      fe_stack_data fe <= o < fe_stack_data fe + bound_stack_data b ->
-      fe_ofs_link fe <= o < fe_ofs_link fe + size_chunk Mptr ->
-      False.
-Proof.
-  clear. intros b fe.
-  generalize (frame_env_separated' b).
-  simpl. intuition.
-  cut (o < o). omega.
-  eapply Z.lt_le_trans.
-  apply H10. etransitivity.
-  2: apply H8.
-  etransitivity. 2: apply align_le ; try omega.
-  etransitivity. 2: apply le_add_pos; [ generalize (bound_local_pos b); omega].
-  etransitivity. 2: apply align_le; try omega.
-  apply size_callee_save_area_incr.
-Qed.
-
 
 Lemma local_callee_save_sep:
   forall b,
@@ -440,13 +367,12 @@ Proof.
   simpl. intuition.
   cut (o < o). omega.
   eapply Z.lt_le_trans.
-  apply H10. etransitivity.
-  2: apply H8.
+  apply H9. etransitivity.
+  2: apply H7.
   etransitivity. 2: apply align_le ; try omega.
   etransitivity. 2: apply le_add_pos; [ generalize (bound_local_pos b); omega].
   apply align_le. omega.
 Qed.
-
 
 Lemma local_arg_sep:
   forall b,
@@ -461,16 +387,14 @@ Proof.
   simpl. intuition.
     cut (o < o). omega.
   eapply Z.lt_le_trans.
-  apply H10. etransitivity.
-  2: apply H8.
+  apply H9. etransitivity.
+  2: apply H7.
   etransitivity. 2: apply align_le ; try omega.
   etransitivity. 2: apply size_callee_save_area_incr.
-  etransitivity. 2: apply le_add_pos; [ destr; omega].
   change fe_ofs_arg with 0.
   rewrite Z.add_0_l.
   apply align_le. destr; omega.
 Qed.
-
 
 Lemma stkdata_arg_sep:
   forall b,
@@ -485,18 +409,16 @@ Proof.
   simpl. intuition.
   cut (o < o). omega.
   eapply Z.lt_le_trans.
-  apply H10. etransitivity.
-  2: apply H8.
+  apply H9. etransitivity.
+  2: apply H7.
   etransitivity. 2: apply align_le ; try omega.
   etransitivity. 2: apply le_add_pos; [ generalize (bound_local_pos b); omega].
   etransitivity. 2: apply align_le ; try omega.
   etransitivity. 2: apply size_callee_save_area_incr.
-  etransitivity. 2: apply le_add_pos; [ destr; omega].
   change fe_ofs_arg with 0.
   rewrite Z.add_0_l.
   apply align_le. destr; omega.
 Qed.
-
 
 Lemma stkdata_local_sep:
   forall b,
@@ -509,31 +431,6 @@ Proof.
   clear. intros b fe.
   generalize (frame_env_separated' b).
   simpl. intuition.
-Qed.
-
-
-
-Lemma retaddr_link_sep:
-  forall b,
-    let fe := make_env b in
-    forall o,
-      fe_ofs_retaddr fe <= o < fe_ofs_retaddr fe + size_chunk Mptr ->
-      fe_ofs_link fe <= o < fe_ofs_link fe + size_chunk Mptr ->
-      False.
-Proof.
-  clear. intros b fe.
-  generalize (frame_env_separated' b).
-  simpl. intuition.
-  cut (o < o). omega.
-  eapply Z.lt_le_trans.
-  apply H10. etransitivity.
-  2: apply H8.
-  etransitivity. 2: apply align_le ; try (destr; omega).
-  etransitivity. 2: apply le_add_pos; [ generalize (bound_stack_data_pos b); omega].
-  etransitivity. 2: apply align_le; try omega.
-  etransitivity. 2: apply le_add_pos; [ generalize (bound_local_pos b); omega].
-  etransitivity. 2: apply align_le; try omega.
-  apply size_callee_save_area_incr.
 Qed.
 
 End WITHMEM.
